Cleaner approach of location in parser

examples/formal-languages/context-free/pegexecScript.sml
@@ -1,6 +1,6 @@
 open HolKernel Parse boolLib bossLib
 
-open boolSimps lcsymtacs
+open boolSimps
 
 open pegTheory locationTheory
 
@@ -13,10 +13,10 @@ val _ = Hol_datatype`
     ksym of ('atok,'bnt,'cvalue) pegsym => kont => kont
   | appf1 of ('cvalue -> 'cvalue) => kont
   | appf2 of ('cvalue -> 'cvalue -> 'cvalue) => kont
-  | returnTo of ('atok # locs) list => ('cvalue # locs) option list => kont
+  | returnTo of ('atok # locs) list => 'cvalue option list => kont
   | poplist of ('cvalue list -> 'cvalue) => kont
   | listsym of ('atok,'bnt,'cvalue) pegsym =>
-               ('cvalue  list -> 'cvalue ) =>
+               ('cvalue list -> 'cvalue) =>
                kont
   | done
   | failed
@@ -28,47 +28,43 @@ val poplist_aux_def = Define`
   poplist_aux acc [] = (acc,[]) (* should never happen *)
 `;
 
-val app_list_locs_def = Define`
-  app_list_locs f l = (f (MAP FST l), merge_list_locs (REVERSE(MAP SND l)))`;
-
-
 val poplistval_def = Define`
-  poplistval f l = 
-    let (values,rest) = poplist_aux [] l in
-      SOME(app_list_locs f values) :: rest `;
-
-
+  poplistval f l = let (values,rest) = poplist_aux [] l
+                   in
+                     SOME(f values) :: rest
+`;
 
 val _ = Hol_datatype `
   evalcase = EV of ('atok,'bnt,'cvalue) pegsym =>
-                   ('atok # locs) list => ('cvalue #locs) option list =>
+                   ('atok # locs) list => 'cvalue option list =>
                    ('atok,'bnt,'cvalue) kont =>
                    ('atok,'bnt,'cvalue) kont
            | AP of ('atok,'bnt,'cvalue) kont =>
-                   ('atok # locs) list => ('cvalue # locs) option list
-           | Result of (('atok # locs)  list # 'cvalue) option # locs
+                   ('atok # locs) list => 'cvalue option list
+           | Result of (('atok # locs) list # 'cvalue) option
            | Looped
 `;
+
 val coreloop_def = zDefine`
   coreloop G =
    OWHILE (λs. case s of Result _ => F
                        | _ => T)
           (λs. case s of
-                   EV (empty v) i r k fk => AP k i (SOME (v, unknown_loc)::r)
+                   EV (empty v) i r k fk => AP k i (SOME v::r)
                  | EV (any tf) i r k fk =>
                    (case i of
                         [] => AP fk i r
-                      | (h, l)::t => AP k t (SOME (tf h, l) :: r))
+                      | h::t => AP k t (SOME (tf h) :: r))
                  | EV (tok P tf2) i r k fk =>
                    (case i of
                         [] => AP fk i r
-                      | (h, l)::t => if P h then AP k t (SOME (tf2 h, l)::r)
+                      | h::t => if P (FST h) then AP k t (SOME (tf2 h)::r)
                                 else AP fk i r)
                  | EV (nt n tf3) i r k fk =>
                    if n ∈ FDOM G.rules then
                      EV (G.rules ' n) i r (appf1 tf3 k) fk
                    else
-                     Result (NONE, unknown_loc)
+                     Result NONE
                  | EV (seq e1 e2 f) i r k fk =>
                      EV e1 i r
                         (ksym e2 (appf2 f k) (returnTo i r fk))
@@ -80,18 +76,17 @@ val coreloop_def = zDefine`
                  | EV (rpt e lf) i r k fk =>
                      EV e i (NONE::r) (listsym e lf k) (poplist lf k)
                  | EV (not e v) i r k fk =>
-                     EV e i r (returnTo i r fk) (returnTo i (SOME (v,unknown_loc)::r) k)
+                     EV e i r (returnTo i r fk) (returnTo i (SOME v::r) k)
                  | AP done i r => Result(case r of
-                                             [] => (NONE, unknown_loc)
-                                           | NONE::t => (NONE, unknown_loc)
-                                           | SOME (rv, l)::t => (SOME(i, rv),l))
-                 | AP failed i r => Result (NONE, unknown_loc)
+                                             [] => NONE
+                                           | NONE::t => NONE
+                                           | SOME rv::t => SOME(i, rv))
+                 | AP failed i r => Result NONE
                  | AP (ksym e k fk) i r => EV e i r k fk
-                 | AP (appf1 f1 k) i (SOME (v,l) :: r) => 
-                     AP k i (SOME (f1 v,l) :: r)
+                 | AP (appf1 f1 k) i (SOME v :: r) => AP k i (SOME (f1 v) :: r)
                  | AP (appf1 _ _) _ _ => Looped
-                 | AP (appf2 f2 k) i (SOME (v1, l1) :: SOME (v2, l2) :: r) =>
-                     AP k i (SOME (f2 v2 v1, merge_locs l2 l1) :: r)
+                 | AP (appf2 f2 k) i (SOME v1 :: SOME v2 :: r) =>
+                     AP k i (SOME (f2 v2 v1) :: r)
                  | AP (appf2 _ _) _ _ => Looped
                  | AP (returnTo i r k) i' r' => AP k i r
                  | AP (listsym e f k) i r =>
@@ -139,10 +134,10 @@ val option_case_COND = prove(
 val better_peg_execs =
     map peg_exec_thm [([`e` |-> `empty v`], []),
                   ([`e` |-> `tok P f`, `i` |-> `[]`], []),
-                  ([`e` |-> `tok P f`, `i` |-> `(x,l)::xs`],
+                  ([`e` |-> `tok P f`, `i` |-> `x::xs`],
                    [Once COND_RAND, option_case_COND]),
                   ([`e` |-> `any f`, `i` |-> `[]`], []),
-                  ([`e` |-> `any f`, `i` |-> `(x,l)::xs`], []),
+                  ([`e` |-> `any f`, `i` |-> `x::xs`], []),
                   ([`e` |-> `seq e1 e2 sf`], []),
                   ([`e` |-> `choice e1 e2 cf`], []),
                   ([`e` |-> `not e v`], []),
@@ -151,8 +146,8 @@ val better_peg_execs =
 val better_apply =
     map (inst_thm applykont_def)
         [([`k` |-> `ksym e k fk`], []),
-         ([`k` |-> `appf1 f k`, `r` |-> `SOME (v,l)::r`], []),
-         ([`k` |-> `appf2 f k`, `r` |-> `SOME (v1,l1)::SOME (v2,l2)::r`], []),
+         ([`k` |-> `appf1 f k`, `r` |-> `SOME v::r`], []),
+         ([`k` |-> `appf2 f k`, `r` |-> `SOME v1::SOME v2::r`], []),
          ([`k` |-> `returnTo i' r' k`], []),
          ([`k` |-> `done`], []),
          ([`k` |-> `failed`], []),
@@ -173,53 +168,43 @@ val _ = app (fn s => ignore (remove_ovl_mapping s {Thy = "pegexec", Name = s}))
             ["AP", "EV"]
 
 val exec_correct0 = prove(
-  ``(∀i e r l l'. peg_eval G (i,e) (r,l,l') ⇒
+  ``(∀i e r. peg_eval G (i,e) r ⇒
              (∀j v k fk stk.
                 r = SOME(j,v) ⇒
-                peg_exec G e i stk k fk = applykont G k j (SOME (v, l, l') :: stk)) ∧
+                peg_exec G e i stk k fk = applykont G k j (SOME v :: stk)) ∧
              (∀k fk stk.
                 r = NONE ⇒ peg_exec G e i stk k fk = applykont G fk i stk)) ∧
-    (∀i e j vlist l l'.
-      peg_eval_list G (i,e) (j,vlist,l,l') ⇒
+    (∀i e j vlist.
+      peg_eval_list G (i,e) (j,vlist) ⇒
       ∀f k stk vs.
-          peg_exec G e i (APPEND (MAP SOME vs) (NONE::stk))
+          peg_exec G e i (MAP SOME vs ++ (NONE::stk))
                      (listsym e f k)
                      (poplist f k) =
-          applykont G k j (SOME (f (APPEND (REVERSE (MAP FST vs)) vlist), 
-                           merge_list_locs ( (MAP SND vs))) :: stk))``,
+          applykont G k j (SOME (f (REVERSE vs ++ vlist)) :: stk))``,
   ho_match_mp_tac peg_eval_strongind' >>
   simp[peg_exec_thm, peg_nt_thm, applykont_thm] >>
   rpt conj_tac
-  >- cheat 
   >- ((* rpt - no elements succeed *)
-      map_every qx_gen_tac [`e`, `f`, `i`, `j`, `vlist`, `l`, `l'`] >> 
-      strip_tac >>
+      map_every qx_gen_tac [`e`, `f`, `i`, `j`, `vlist`] >> strip_tac >>
       map_every qx_gen_tac [`k`, `stk`] >>
       first_x_assum (qspecl_then [`f`, `k`, `stk`, `[]`] mp_tac) >>
-      simp[merge_list_locs_def] >>
-      cheat 
-      )
+      simp[])
   >- ((* poplistval works *)
       rpt strip_tac >> rpt AP_TERM_TAC >> rpt (pop_assum (K ALL_TAC)) >>
-      simp[poplistval_def, app_list_locs_def,MAP_REVERSE] >>
-(*      qmatch_abbrev_tac `
-        (λ(values,rest). SOME (app_list_locs f values)::rest)
+      simp[poplistval_def] >>
+      qmatch_abbrev_tac `
+        (λ(values,rest). SOME (f values)::rest)
         (poplist_aux [] (MAP SOME vs ++ [NONE] ++ stk)) =
-        SOME (f (REVERSE (MAP FST vs), i, e'))::stk` >> *)
+        SOME (f (REVERSE vs))::stk` >>
       qsuff_tac `∀a. poplist_aux a (MAP SOME vs ++ [NONE] ++ stk) =
-                     (REVERSE vs ++ a, stk)`
-                     >- simp[MAP_REVERSE] 
-      >- (Induct_on `vs` >> simp[poplist_aux_def]))
+                     (REVERSE vs ++ a, stk)` >- simp[] >>
+      Induct_on `vs` >> simp[poplist_aux_def])
   >- ((* rpt - some elements succeed *)
-      map_every qx_gen_tac [`e`,`i0`,`i1`,`l1`,`l2`,`j`,`l3`,`l4`,`v`,`s`] >> 
-      strip_tac >>
+      map_every qx_gen_tac [`e`, `i0`, `i1`, `j`, `v`, `vs`] >> strip_tac >>
       map_every qx_gen_tac [`f`, `k`, `stk`, `vs'`] >>
-      first_x_assum (qspecl_then [`f`, `k`, `stk`, `(v, l1, l2)::vs'`] mp_tac) >>
+      first_x_assum (qspecl_then [`f`, `k`, `stk`, `v::vs'`] mp_tac) >>
       simp[] >>
-      simp_tac bool_ss [GSYM
-          listTheory.APPEND_ASSOC,listTheory.APPEND,merge_locs_def] >>
-      cheat
-      ))
+      simp_tac bool_ss [GSYM listTheory.APPEND_ASSOC, listTheory.APPEND]))
 
 val exec_correct = save_thm(
   "exec_correct",
@@ -243,25 +228,21 @@ val list_CASES = listTheory.list_CASES
 
 val pegexec = store_thm(
   "pegexec",
-  ``peg_eval G (s,e) (r,l) ⇒ ?l'. peg_exec G e s [] done failed = Result (r,l')``,
-   metis_tac [option_CASES, pair_CASES, pegexec_fails, pegexec_succeeds]);
+  ``peg_eval G (s,e) r ⇒ peg_exec G e s [] done failed = Result r``,
+  metis_tac [option_CASES, pair_CASES, pegexec_fails, pegexec_succeeds]);
 
 val peg_eval_executed = store_thm(
   "peg_eval_executed",
   ``wfG G ∧ e ∈ Gexprs G ⇒
-    (peg_eval G (s,e) (r,l) ⇔ ?l'. peg_exec G e s [] done failed = Result (r,l'))``,
+    (peg_eval G (s,e) r ⇔ peg_exec G e s [] done failed = Result r)``,
   strip_tac >> eq_tac
-  >- (
-    `r = NONE ∨ ∃s' v. r = SOME (s',v)`
+  >- (`r = NONE ∨ ∃s' v. r = SOME (s',v)`
         by metis_tac[option_CASES, pair_CASES] >>
-      simp[pegexec_fails, pegexec_succeeds] >> metis_tac[pegexec]) >>
+      simp[pegexec_fails, pegexec_succeeds]) >>
   strip_tac >>
-  `∃r' l''. peg_eval G (s,e) (r',l'')` by metis_tac[peg_eval_total] >>
-  Cases_on `l''` >>
+  `∃r'. peg_eval G (s,e) r'` by metis_tac[peg_eval_total] >>
   first_assum (assume_tac o MATCH_MP (CONJUNCT1 peg_deterministic)) >>
-  first_x_assum (assume_tac o MATCH_MP pegexec) >> fs[] >>
-  fs[] >>
-  cheat );
+  simp[] >> first_x_assum (assume_tac o MATCH_MP pegexec) >> fs[]);
 
 val destResult_def = Define`destResult (Result r) = r`
 val _ = export_rewrites ["destResult_def"]
@@ -269,43 +250,41 @@ val _ = export_rewrites ["destResult_def"]
 val pegparse_def = Define`
   pegparse G s =
     if wfG G then destResult (peg_exec G G.start s [] done failed)
-    else (NONE, unknown_loc) `;
+    else NONE
+`;
 
 val pegparse_eq_SOME = store_thm(
   "pegparse_eq_SOME",
-  ``pegparse G s = (SOME (s',v),l) ⇔ wfG G ∧ peg_eval G (s,G.start) (SOME(s',v), l)``,
+  ``pegparse G s = SOME (s',v) ⇔ wfG G ∧ peg_eval G (s,G.start) (SOME(s',v))``,
   Tactical.REVERSE (Cases_on `wfG G`) >- simp[pegparse_def] >>
   `∃r. peg_eval G (s,G.start) r`
     by metis_tac [peg_eval_total, start_IN_Gexprs] >>
-  Cases_on`r` >> Cases_on`r'` >>
   first_assum (assume_tac o MATCH_MP (CONJUNCT1 peg_deterministic)) >>
   simp[] >>
-  `q = NONE ∨ ∃s2 v2. q = SOME (s2,v2)` by metis_tac [option_CASES, pair_CASES]
+  `r = NONE ∨ ∃s2 v2. r = SOME (s2,v2)` by metis_tac [option_CASES, pair_CASES]
   >- rw[pegparse_def, pegexec_fails] >>
   rw[pegparse_def] >> first_x_assum (assume_tac o MATCH_MP pegexec_succeeds) >>
   simp[] >> metis_tac[]);
 
 val pegparse_eq_NONE = store_thm(
   "pegparse_eq_NONE",
-  ``pegparse G s = (NONE,unknown_loc) ⇔ ? l. ¬wfG G ∨ peg_eval G (s,G.start) (NONE,l)``,
+  ``pegparse G s = NONE ⇔ ¬wfG G ∨ peg_eval G (s,G.start) NONE``,
   Cases_on `wfG G` >> simp[pegparse_def] >>
   `∃r. peg_eval G (s,G.start) r`
     by metis_tac [peg_eval_total, start_IN_Gexprs] >>
-  Cases_on`r` >> Cases_on`r'` >>
   first_assum (assume_tac o MATCH_MP (CONJUNCT1 peg_deterministic)) >>
   simp[] >>
-  `q = NONE ∨ ∃s2 v2. q = SOME (s2,v2)` by metis_tac [option_CASES, pair_CASES]
+  `r = NONE ∨ ∃s2 v2. r = SOME (s2,v2)` by metis_tac [option_CASES, pair_CASES]
   >- rw[pegexec_fails] >>
   rw[] >> first_x_assum (assume_tac o MATCH_MP pegexec_succeeds) >>
   simp[]);
 
 val peg_exec_total = store_thm(
   "peg_exec_total",
-  ``wfG G ==> ∃r l. peg_exec G G.start i [] done failed = Result (r, l)``,
+  ``wfG G ==> ∃r. peg_exec G G.start i [] done failed = Result r``,
   strip_tac >>
-  `∃pr l. peg_eval G (i, G.start) (pr,l)` by simp[peg_eval_total, start_IN_Gexprs] >>
-  pop_assum mp_tac >> 
-  simp[peg_eval_executed, start_IN_Gexprs] >> rw[] >> rw[]);
+  `∃pr. peg_eval G (i, G.start) pr` by simp[peg_eval_total, start_IN_Gexprs] >>
+  pop_assum mp_tac >> simp[peg_eval_executed, start_IN_Gexprs]);
 
 val option_case_EQ = prove(
   ``option_CASE x n s = v ⇔ x = NONE ∧ n = v ∨ ∃v0. x = SOME v0 ∧ v = s v0``,
@@ -322,3 +301,4 @@ val coreloop_total = save_thm(
 
 
 val _ = export_theory()
+
