examples/formal-languages/context-free/pegScript.sml
@@ -13,10 +13,10 @@ val _ = new_theory "peg"
 
 val _ = Hol_datatype `pegsym =
     empty of 'c
-  | any of ('a -> 'c)
-  | tok of ('a -> bool) => ('a -> 'c)
+  | any of (('a # locs) -> 'c)
+  | tok of ('a -> bool) => (('a # locs) -> 'c)
   | nt of 'b inf => ('c -> 'c)
-  | seq of pegsym => pegsym => ('c -> 'c -> 'c)
+  | seq of pegsym => pegsym => ('c  -> 'c -> 'c)
   | choice of pegsym => pegsym => ('c + 'c -> 'c)
   | rpt of pegsym => ('c list -> 'c)
   | not of pegsym => 'c
@@ -26,67 +26,64 @@ val _ = Hol_datatype`
   peg = <| start : ('a,'b,'c) pegsym ;
            rules : 'b inf |-> ('a,'b,'c) pegsym |>
 `
-
+(* Option type should be replaced with sum type (loc. for NONE *)
 val (peg_eval_rules, peg_eval_ind, peg_eval_cases) = Hol_reln`
-  (∀s c. peg_eval G (s, empty c) (SOME(s, c), unknown_loc)) ∧
-  (∀n l r s f c.
-       n ∈ FDOM G.rules ∧ peg_eval G (s, G.rules ' n) (SOME(r, c), l) ⇒
-       peg_eval G (s, nt n f) (SOME(r, f c), l)) ∧
-  (∀n l s f.
-       n ∈ FDOM G.rules ∧ peg_eval G (s, G.rules ' n) (NONE, l) ⇒
-           peg_eval G (s, nt n f) (NONE, l)) ∧
-  (∀h l t f. peg_eval G ((h, l)::t, any f) (SOME (t, f h), l)) ∧
-  (∀f. peg_eval G ([], any f) (NONE, unknown_loc)) ∧
-  (∀e l t P f. P e ⇒ peg_eval G ((e, l)::t, tok P f) (SOME(t, f e), l)) ∧
-  (∀e l t P f. ¬P e ⇒ peg_eval G ((e, l)::t, tok P f) (NONE, l)) ∧
-  (∀P f. peg_eval G ([], tok P f) (NONE, unknown_loc)) ∧
-  (∀e l s c. peg_eval G (s, e) (NONE, l) ⇒ 
-             peg_eval G (s, not e c) (SOME(s,c),l)) ∧
-  (∀e l s s' c. peg_eval G (s, e) (SOME s', l) ⇒ peg_eval G (s, not e c) (NONE, l))  ∧
-  (∀e1 l1 e2 s f. peg_eval G (s, e1) (NONE, l1) ⇒ 
-                  peg_eval G (s, seq e1 e2 f) (NONE, l1))  ∧
-  (∀e1 l1 e2 l2 s0 s1 c1 f.
-     peg_eval G (s0, e1) (SOME (s1, c1), l1) ∧ peg_eval G (s1, e2) (NONE, l2) ⇒
-     peg_eval G (s0, seq e1 e2 f) (NONE, l2)) ∧
-  (∀e1 l1 e2 l2 s0 s1 s2 c1 c2 f.
-     peg_eval G (s0, e1) (SOME(s1, c1), l1) ∧
-     peg_eval G (s1, e2) (SOME(s2, c2), l2) ⇒
-     peg_eval G (s0, seq e1 e2 f) (SOME(s2, f c1 c2), merge_locs l1 l2)) ∧
-  (∀e1 l1 e2 l2 s f.
-     peg_eval G (s, e1) (NONE, l1) ∧ peg_eval G (s, e2) (NONE, l2) ⇒
-     peg_eval G (s, choice e1 e2 f) (NONE, l2)) ∧
-  (∀e1 l1 e2 s s' f c.
-     peg_eval G (s, e1) (SOME(s',c), l1) ⇒
-     peg_eval G (s, choice e1 e2 f) (SOME(s', f (INL c)), l1)) ∧
-  (∀e1 l1 e2 l2 s s' f c.
-     peg_eval G (s, e1) (NONE, l1) ∧ peg_eval G (s, e2) (SOME(s',c), l2) ⇒
-     peg_eval G (s, choice e1 e2 f) (SOME(s',f (INR c)),l2))  ∧
-  (∀e f s s1 list l.
-     peg_eval_list G (s, e) (s1,list, l) ⇒
-     peg_eval G (s, rpt e f) (SOME(s1, f list), l)) ∧
-  (∀e l s. peg_eval G (s, e) (NONE, l) ⇒ peg_eval_list G (s, e) (s,[],l)) ∧
-  (∀e s0 s1 l1 s2 l2 c cs.
-     peg_eval G (s0, e) (SOME(s1,c), l1) ∧
-     peg_eval_list G (s1, e) (s2,cs, l2) ⇒
-     peg_eval_list G (s0, e) (s2,c::cs, merge_locs l1 l2))
+  (∀s c. peg_eval G (s, empty c) (SOME(s, c))) ∧
+  (∀n r s f c.
+       n ∈ FDOM G.rules ∧ peg_eval G (s, G.rules ' n) (SOME(r,c)) ⇒
+       peg_eval G (s, nt n f) (SOME(r, f c))) ∧
+  (∀n s f.
+       n ∈ FDOM G.rules ∧ peg_eval G (s, G.rules ' n) NONE ⇒
+       peg_eval G (s, nt n f) NONE) ∧
+  (∀h t f. peg_eval G (h::t, any f) (SOME (t, f h))) ∧
+  (∀f. peg_eval G ([], any f) NONE) ∧
+  (∀e t P f. P (FST e) ⇒ peg_eval G (e::t, tok P f) (SOME(t, f e))) ∧
+  (∀e t P f. ¬P (FST e) ⇒ peg_eval G (e::t, tok P f) NONE) ∧
+  (∀P f. peg_eval G ([], tok P f) NONE) ∧
+  (∀e s c. peg_eval G (s, e) NONE ⇒ peg_eval G (s, not e c) (SOME(s,c))) ∧
+  (∀e s s' c. peg_eval G (s, e) (SOME s') ⇒ peg_eval G (s, not e c) NONE)  ∧
+  (∀e1 e2 s f. peg_eval G (s, e1) NONE ⇒ peg_eval G (s, seq e1 e2 f) NONE)  ∧
+  (∀e1 e2 s0 s1 c1 f.
+     peg_eval G (s0, e1) (SOME (s1, c1)) ∧ peg_eval G (s1, e2) NONE ⇒
+     peg_eval G (s0, seq e1 e2 f) NONE) ∧
+  (∀e1 e2 s0 s1 s2 c1 c2 f.
+     peg_eval G (s0, e1) (SOME(s1, c1)) ∧
+     peg_eval G (s1, e2) (SOME(s2, c2)) ⇒
+     peg_eval G (s0, seq e1 e2 f) (SOME(s2, f c1 c2))) ∧
+  (∀e1 e2 s f.
+     peg_eval G (s, e1) NONE ∧ peg_eval G (s, e2) NONE ⇒
+     peg_eval G (s, choice e1 e2 f) NONE) ∧
+  (∀e1 e2 s s' f c.
+     peg_eval G (s, e1) (SOME(s',c)) ⇒
+     peg_eval G (s, choice e1 e2 f) (SOME(s', f (INL c)))) ∧
+  (∀e1 e2 s s' f c.
+     peg_eval G (s, e1) NONE ∧ peg_eval G (s, e2) (SOME(s',c)) ⇒
+     peg_eval G (s, choice e1 e2 f) (SOME(s',f (INR c))))  ∧
+  (∀e f s s1 list.
+     peg_eval_list G (s, e) (s1,list) ⇒
+     peg_eval G (s, rpt e f) (SOME(s1, f list))) ∧
+  (∀e s. peg_eval G (s, e) NONE ⇒ peg_eval_list G (s, e) (s,[])) ∧
+  (∀e s0 s1 s2 c cs.
+     peg_eval G (s0, e) (SOME(s1,c)) ∧
+     peg_eval_list G (s1, e) (s2,cs) ⇒
+     peg_eval_list G (s0, e) (s2,c::cs))
 `;
 
 val peg_eval_strongind' = save_thm(
   "peg_eval_strongind'",
   theorem "peg_eval_strongind"
-    |> SIMP_RULE (srw_ss()) [pairTheory.FORALL_PROD]
-    |> Q.SPECL [`G`, `\es0 r. P1 (FST es0) (SND es0) (FST r) (SND r)`,
-    `\es0 sr. P2 (FST es0) (SND es0) (FST sr) ((FST o SND) sr) ((SND o SND) sr)`]
- |> SIMP_RULE (srw_ss()) [])
+             |> SIMP_RULE (srw_ss()) [pairTheory.FORALL_PROD]
+             |> Q.SPECL [`G`, `\es0 r. P1 (FST es0) (SND es0) r`,
+                         `\es0 sr. P2 (FST es0) (SND es0) (FST sr) (SND sr)`]
+             |> SIMP_RULE (srw_ss()) [])
 
 open rich_listTheory
 val peg_eval_suffix0 = prove(
-  ``(∀s0 e sr l l'. peg_eval G (s0,e) (sr,l, l') ⇒ ∀s r. sr = SOME (s,r) ⇒ IS_SUFFIX s0 s) ∧
-    ∀s0 e s rl l l'. peg_eval_list G (s0,e) (s,rl,l,l') ⇒ IS_SUFFIX s0 s``,
-  HO_MATCH_MP_TAC peg_eval_strongind' 
-  THEN SRW_TAC [][IS_SUFFIX_compute, IS_PREFIX_APPEND3,
-                                       IS_PREFIX_REFL]
-  THEN METIS_TAC [IS_PREFIX_TRANS]);
+  ``(∀s0 e sr. peg_eval G (s0,e) sr ⇒ ∀s r. sr = SOME (s,r) ⇒ IS_SUFFIX s0 s) ∧
+    ∀s0 e s rl. peg_eval_list G (s0,e) (s,rl) ⇒ IS_SUFFIX s0 s``,
+  HO_MATCH_MP_TAC peg_eval_strongind' THEN SRW_TAC [][IS_SUFFIX_compute, IS_PREFIX_APPEND3,
+                                       IS_PREFIX_REFL] THEN
+  METIS_TAC [IS_PREFIX_TRANS]);
 
 (* Theorem 3.1 *)
 val peg_eval_suffix = save_thm(
@@ -96,26 +93,21 @@ val peg_eval_suffix = save_thm(
 (* Theorem 3.2 *)
 val peg_deterministic = store_thm(
   "peg_deterministic",
-  ``(∀s0 e sr l1 l2. peg_eval G (s0,e) (sr,l1,l2) 
-     ⇒ ∀sr'. peg_eval G (s0,e) sr' 
-     ⇔ sr' = (sr,l1,l2)) ∧
-    ∀s0 e s rl l l'. peg_eval_list G (s0,e) (s,rl,l,l') ⇒
-              ∀srl'. peg_eval_list G (s0,e) srl' ⇔ srl' = (s,rl,l,l')``,
+  ``(∀s0 e sr. peg_eval G (s0,e) sr ⇒ ∀sr'. peg_eval G (s0,e) sr' ⇔ sr' = sr) ∧
+    ∀s0 e s rl. peg_eval_list G (s0,e) (s,rl) ⇒
+                ∀srl'. peg_eval_list G (s0,e) srl' ⇔ srl' = (s,rl)``,
   HO_MATCH_MP_TAC peg_eval_strongind' THEN SRW_TAC [][] THEN
   ONCE_REWRITE_TAC [peg_eval_cases] THEN SRW_TAC [][]);
 
 (* Lemma 3.3 *)
 val peg_badrpt = store_thm(
   "peg_badrpt",
-  ``peg_eval G (s0,e) (SOME(s0,r),l) ⇒ ∀r' l'. ¬peg_eval G (s0, rpt e f) (r', l')``,
-  strip_tac >> 
-  simp[Once peg_eval_cases] 
-  >> map_every qx_gen_tac [`l'`, `s1`, `l1`] >>
-  Cases_on `l'` >>
+  ``peg_eval G (s0,e) (SOME(s0,r)) ⇒ ∀r. ¬peg_eval G (s0, rpt e f) r``,
+  strip_tac >> simp[Once peg_eval_cases] >> map_every qx_gen_tac [`s1`, `l`] >>
   disch_then (assume_tac o MATCH_MP (CONJUNCT2 peg_deterministic)) >>
-  `peg_eval_list G (s0,e) (s1,r::l1,merge_locs l (q,r'))`
-    by METIS_TAC [pairTheory.pair_CASES, last (peg_eval_rules |> SPEC_ALL |> CONJUNCTS)] >>
-  pop_assum mp_tac >> simp[]); 
+  `peg_eval_list G (s0,e) (s1,r::l)`
+    by METIS_TAC [last (peg_eval_rules |> SPEC_ALL |> CONJUNCTS)] >>
+  pop_assum mp_tac >> simp[]);
 
 val (peg0_rules, peg0_ind, peg0_cases) = Hol_reln`
   (∀c. peg0 G (empty c)) ∧
@@ -163,17 +155,18 @@ val (peg0_rules, peg0_ind, peg0_cases) = Hol_reln`
 
 val peg_eval_suffix' = store_thm(
   "peg_eval_suffix'",
-  ``peg_eval G (s0,e) (SOME(s,c), l,l') ⇒
+  ``peg_eval G (s0,e) (SOME(s,c)) ⇒
     s0 = s ∨ IS_SUFFIX s0 s ∧ LENGTH s < LENGTH s0``,
   strip_tac >> imp_res_tac peg_eval_suffix >> Cases_on `s0 = s` >- simp[] >>
-  fs[IS_SUFFIX_compute] >> imp_res_tac IS_PREFIX_LENGTH >> fs[] >>
+  fs[IS_SUFFIX_compute] >>
+  imp_res_tac IS_PREFIX_LENGTH >> fs[] >>
   qsuff_tac `LENGTH s ≠ LENGTH s0` >- (strip_tac >> decide_tac) >>
   strip_tac >>
   metis_tac [IS_PREFIX_LENGTH_ANTI, LENGTH_REVERSE, REVERSE_REVERSE]);
 
 val peg_eval_list_suffix' = store_thm(
   "peg_eval_list_suffix'",
-  ``peg_eval_list G (s0, e) (s,rl,l,l') ⇒
+  ``peg_eval_list G (s0, e) (s,rl) ⇒
     s0 = s ∨ IS_SUFFIX s0 s ∧ LENGTH s < LENGTH s0``,
   strip_tac >> imp_res_tac peg_eval_suffix >> Cases_on `s0 = s` >- simp[] >>
   fs[IS_SUFFIX_compute] >> imp_res_tac IS_PREFIX_LENGTH >> fs[] >>
@@ -185,11 +178,11 @@ fun rule_match th = FIRST (List.mapPartial (total MATCH_MP_TAC)
                                            (th |> SPEC_ALL |> CONJUNCTS))
 
 val lemma4_1a0 = prove(
-  ``(∀s0 e r l l'. peg_eval G (s0, e) (r,l, l') ⇒
+  ``(∀s0 e r. peg_eval G (s0, e) r ⇒
               (∀c. r = SOME(s0,c) ⇒ peg0 G e) ∧
               (r = NONE ⇒ pegfail G e) ∧
               (∀s c. r = SOME(s,c) ∧ LENGTH s < LENGTH s0 ⇒ peggt0 G e)) ∧
-    (∀s0 e s rl l l'. peg_eval_list G (s0,e) (s,rl,l,l') ⇒
+    (∀s0 e s rl. peg_eval_list G (s0,e) (s,rl) ⇒
                  (s0 = s ⇒ pegfail G e) ∧
                  (LENGTH s < LENGTH s0 ⇒ peggt0 G e))``,
   ho_match_mp_tac peg_eval_strongind' >> simp[peg0_rules] >> rpt conj_tac
@@ -201,11 +194,10 @@ val lemma4_1a0 = prove(
       imp_res_tac peg_eval_suffix' >> fs[] >> rw[] >>
       full_simp_tac (srw_ss() ++ ARITH_ss) []) >>
   rpt strip_tac
-  >- (
-      first_x_assum match_mp_tac >> rw[] >>
+  >- (first_x_assum match_mp_tac >> rw[] >>
       imp_res_tac peg_eval_suffix >> fs[IS_SUFFIX_compute] >>
       imp_res_tac IS_PREFIX_LENGTH >> fs[] >>
-      `LENGTH s1 = LENGTH s0` by decide_tac >>
+      `LENGTH s = LENGTH s0'` by decide_tac >>
       metis_tac [IS_PREFIX_LENGTH_ANTI, LENGTH_REVERSE, REVERSE_REVERSE]) >>
   imp_res_tac peg_eval_suffix' >- rw[] >>
   imp_res_tac peg_eval_list_suffix' >- rw[] >>
@@ -282,20 +274,19 @@ val list_CASES = listTheory.list_CASES
 
 val reducing_peg_eval_makes_list = prove(
   ``(∀s. LENGTH s < n ⇒ ∃r. peg_eval G (s, e) r) ∧ ¬peg0 G e ∧ LENGTH s0 < n ⇒
-    ∃s' rl l. peg_eval_list G (s0,e) (s',rl,l)``,
+    ∃s' rl. peg_eval_list G (s0,e) (s',rl)``,
   strip_tac >> completeInduct_on `LENGTH s0` >> rw[] >>
   full_simp_tac (srw_ss() ++ DNF_ss ++ ARITH_ss) [] >>
-  `∃l. peg_eval G (s0,e) (NONE,l) ∨ ∃s1 c. peg_eval G (s0,e) (SOME(s1,c),l)`
+  `peg_eval G (s0,e) NONE ∨ ∃s1 c. peg_eval G (s0,e) (SOME(s1,c))`
     by metis_tac [pair_CASES, option_CASES]
   >- metis_tac [peg_eval_rules] >>
-  Cases_on `l` >>
   `s0 ≠ s1` by metis_tac [lemma4_1a] >>
   `LENGTH s1 < LENGTH s0` by metis_tac [peg_eval_suffix'] >>
   metis_tac [peg_eval_rules]);
 
 val peg_eval_total = store_thm(
   "peg_eval_total",
-  ``wfG G ⇒ ∀s e. e ∈ Gexprs G ⇒ ∃r l. peg_eval G (s,e) (r,l)``,
+  ``wfG G ⇒ ∀s e. e ∈ Gexprs G ⇒ ∃r. peg_eval G (s,e) r``,
   simp[wfG_def] >> strip_tac >> gen_tac >>
   completeInduct_on `LENGTH s` >>
   full_simp_tac (srw_ss() ++ DNF_ss) [] >> rpt strip_tac >>
@@ -309,20 +300,18 @@ val peg_eval_total = store_thm(
       asm_simp_tac (srw_ss() ++ DNF_ss) [Gexprs_def, FRANGE_DEF] >>
       metis_tac [subexprs_included])
   >- (* empty *) metis_tac [peg_eval_rules]
-  >- (* any *) metis_tac [peg_eval_rules, pair_CASES, list_CASES]
-  >- (* tok *) metis_tac [peg_eval_rules, pair_CASES, list_CASES]
+  >- (* any *) metis_tac [peg_eval_rules, list_CASES]
+  >- (* tok *) metis_tac [peg_eval_rules, list_CASES]
   >- (* not *) metis_tac [peg_eval_rules, optionTheory.option_nchotomy,
                           IN_Gexprs_E]
-  >- ((* seq *) 
-  Q.MATCH_ASSUM_ABBREV_TAC `seq e1 e2 f ∈ Gexprs G` >>
+  >- ((* seq *) Q.MATCH_ASSUM_ABBREV_TAC `seq e1 e2 f ∈ Gexprs G` >>
       markerLib.RM_ALL_ABBREVS_TAC >>
       `e1 ∈ Gexprs G` by imp_res_tac IN_Gexprs_E >>
-      `∃l. peg_eval G (s,e1) (NONE,l) ∨ ∃s' c. peg_eval G (s,e1) (SOME(s',c),l)`
+      `peg_eval G (s,e1) NONE ∨ ∃s' c. peg_eval G (s,e1) (SOME(s',c))`
         by metis_tac[option_CASES, pair_CASES]
       >- metis_tac [peg_eval_rules] >>
-      Cases_on `l` >>
       Cases_on `s' = s`
-      >- ( `peg0 G e1` by metis_tac [lemma4_1a] >>
+      >- (`peg0 G e1` by metis_tac [lemma4_1a] >>
           `e2 ∈ Gexprs G` by imp_res_tac IN_Gexprs_E >>
           metis_tac [peg_eval_rules, option_CASES, pair_CASES]) >>
       `LENGTH s' < LENGTH s` by metis_tac [peg_eval_suffix'] >>
@@ -331,11 +320,10 @@ val peg_eval_total = store_thm(
   >- (* choice *)
      metis_tac [peg_eval_rules, option_CASES, IN_Gexprs_E, pair_CASES] >>
   (* rpt *) imp_res_tac IN_Gexprs_E >>
-  `∃l. peg_eval G (s, e) (NONE,l) ∨ ∃s' c. peg_eval G (s,e) (SOME (s',c),l)`
+  `peg_eval G (s, e) NONE ∨ ∃s' c. peg_eval G (s,e) (SOME (s',c))`
     by metis_tac [option_CASES, pair_CASES]
-  >- (`∃l. peg_eval_list G (s,e) (s,[],l)` by metis_tac [peg_eval_rules] >>
+  >- (`peg_eval_list G (s,e) (s,[])` by metis_tac [peg_eval_rules] >>
       metis_tac [peg_eval_rules]) >>
-      Cases_on `l` >>
   `s' ≠ s` by metis_tac [lemma4_1a] >>
   `LENGTH s' < LENGTH s` by metis_tac [peg_eval_suffix'] >>
   metis_tac [peg_eval_rules, reducing_peg_eval_makes_list])
@@ -366,79 +354,79 @@ val checkAhead_def = Define`
 
 val peg_eval_seq_SOME = store_thm(
   "peg_eval_seq_SOME",
-  ``peg_eval G (i0, seq s1 s2 f) (SOME (i,r),l) ⇔
-    ∃i1 r1 r2 l1 l2. peg_eval G (i0, s1) (SOME (i1,r1),l1) ∧
-               peg_eval G (i1, s2) (SOME (i,r2),l2) ∧ (r = f r1 r2)∧
-               l = merge_locs l1 l2``,
+  ``peg_eval G (i0, seq s1 s2 f) (SOME (i,r)) ⇔
+    ∃i1 r1 r2. peg_eval G (i0, s1) (SOME (i1,r1)) ∧
+               peg_eval G (i1, s2) (SOME (i,r2)) ∧ (r = f r1 r2)``,
   simp[Once peg_eval_cases] >> metis_tac[]);
 
 val peg_eval_seq_NONE = store_thm(
   "peg_eval_seq_NONE",
-  ``peg_eval G (i0, seq s1 s2 f) (NONE,l) ⇔
-      peg_eval G (i0, s1) (NONE,l) ∨
-      ∃i r l'. peg_eval G (i0,s1) (SOME(i,r),l') ∧
-            peg_eval G (i,s2) (NONE,l)``,
+  ``peg_eval G (i0, seq s1 s2 f) NONE ⇔
+      peg_eval G (i0, s1) NONE ∨
+      ∃i r. peg_eval G (i0,s1) (SOME(i,r)) ∧
+            peg_eval G (i,s2) NONE``,
   simp[Once peg_eval_cases] >> metis_tac[]);
 
 val peg_eval_tok_NONE = save_thm(
   "peg_eval_tok_NONE",
-  ``peg_eval G (i, tok P f) (NONE,l)``
+  ``peg_eval G (i, tok P f) NONE``
     |> SIMP_CONV (srw_ss()) [Once peg_eval_cases])
 
 val peg_eval_tok_SOME = store_thm(
   "peg_eval_tok_SOME",
-  ``peg_eval G (i0, tok P f) (SOME (i,r),l) ⇔ ∃h. P h ∧ i0 = (h,l)::i ∧ r = f h``,
+  ``peg_eval G (i0, tok P f) (SOME (i,r)) ⇔ ∃h. P (FST h) ∧ i0 = h::i ∧ r = f h``,
   simp[Once peg_eval_cases] >> metis_tac[]);
 
 val peg_eval_empty = store_thm(
   "peg_eval_empty[simp]",
-  ``peg_eval G (i, empty r) x ⇔ (x = (SOME(i,r),unknown_loc))``,
+  ``peg_eval G (i, empty r) x ⇔ (x = SOME(i,r))``,
   simp[Once peg_eval_cases])
 
 val peg_eval_NT_SOME = store_thm(
   "peg_eval_NT_SOME",
-  ``peg_eval G (i0,nt N f) (SOME(i,r),l) ⇔
+  ``peg_eval G (i0,nt N f) (SOME(i,r)) ⇔
       ∃r0. r = f r0 ∧ N ∈ FDOM G.rules ∧
-           peg_eval G (i0,G.rules ' N) (SOME(i,r0),l)``,
+           peg_eval G (i0,G.rules ' N) (SOME(i,r0))``,
   simp[Once peg_eval_cases]);
 
 val peg_eval_choice = store_thm(
   "peg_eval_choice",
-  ``∀x l.
-     peg_eval G (i0, choice s1 s2 f) (x,l) ⇔
-      (∃i r. peg_eval G (i0, s1) (SOME(i, r),l) ∧ x = SOME(i, f (INL r))) ∨
-      (∃i r l'. peg_eval G (i0, s1) (NONE,l') ∧
-             peg_eval G (i0, s2) (SOME(i, r),l) ∧ x = SOME(i, f (INR r))) ∨
-       ∃ l'.peg_eval G (i0, s1) (NONE,l') ∧ peg_eval G (i0,s2) (NONE,l) ∧ (x = NONE)``,
+  ``∀x.
+     peg_eval G (i0, choice s1 s2 f) x ⇔
+      (∃i r. peg_eval G (i0, s1) (SOME(i, r)) ∧ x = SOME(i, f (INL r))) ∨
+      (∃i r. peg_eval G (i0, s1) NONE ∧
+             peg_eval G (i0, s2) (SOME(i, r)) ∧ x = SOME(i, f (INR r))) ∨
+      peg_eval G (i0, s1) NONE ∧ peg_eval G (i0,s2) NONE ∧ (x = NONE)``,
   simp[Once peg_eval_cases, SimpLHS] >>
   simp[optionTheory.FORALL_OPTION, pairTheory.FORALL_PROD] >> metis_tac[]);
 
 val peg_eval_choicel_NIL = store_thm(
   "peg_eval_choicel_NIL[simp]",
-  ``peg_eval G (i0, choicel []) (x, unknown_loc) = (x = NONE)``,
+  ``peg_eval G (i0, choicel []) x = (x = NONE)``,
   simp[choicel_def, Once peg_eval_cases]);
 
 val peg_eval_choicel_CONS = store_thm(
   "peg_eval_choicel_CONS",
-  ``∀x l. peg_eval G (i0, choicel (h::t)) (x,l) ⇔
-          peg_eval G (i0, h) (x,l) ∧ x <> NONE ∨
-          ∃ l'.peg_eval G (i0,h) (NONE,l') ∧ peg_eval G (i0, choicel t) (x,l)``,
+  ``∀x. peg_eval G (i0, choicel (h::t)) x ⇔
+          peg_eval G (i0, h) x ∧ x <> NONE ∨
+          peg_eval G (i0,h) NONE ∧ peg_eval G (i0, choicel t) x``,
   simp[choicel_def, SimpLHS, Once peg_eval_cases] >>
   simp[pairTheory.FORALL_PROD, optionTheory.FORALL_OPTION]);
 
 val peg_eval_rpt = store_thm(
   "peg_eval_rpt",
-  ``peg_eval G (i0, rpt s f) (x,l) ⇔
-      ∃i li. peg_eval_list G (i0,s) (i,li,l) ∧ x = SOME(i,f li)``,
+  ``peg_eval G (i0, rpt s f) x ⇔
+      ∃i l. peg_eval_list G (i0,s) (i,l) ∧ x = SOME(i,f l)``,
   simp[Once peg_eval_cases, SimpLHS] >> metis_tac[]);
 
 val peg_eval_list = Q.store_thm(
   "peg_eval_list",
-  `peg_eval_list G (i0, e) (i, r, l) ⇔
-     peg_eval G (i0, e) (NONE, l) ∧ i = i0 ∧ r = [] ∨
-     (∃i1 rh rt l1 l2.
-        peg_eval G (i0, e) (SOME (i1, rh),l1) ∧
-        peg_eval_list G (i1, e) (i, rt,l2) ∧ r = rh::rt ∧ l = merge_locs l1 l2)`,
+  `peg_eval_list G (i0, e) (i, r) ⇔
+     peg_eval G (i0, e) NONE ∧ i = i0 ∧ r = [] ∨
+     (∃i1 rh rt.
+        peg_eval G (i0, e) (SOME (i1, rh)) ∧
+        peg_eval_list G (i1, e) (i, rt) ∧ r = rh::rt)`,
   simp[Once peg_eval_cases, SimpLHS] >> metis_tac[]);
 
 val _ = export_theory()
+
